src/program_proof/pav/msv.v
@@ -16,27 +16,26 @@ this difference is why we separated the "history" and "latest" resources. *)
 Section proof.
 Context `{!heapGS Σ, !pavG Σ}.
 
-Definition msv_Some (m : adtr_map_ty) vrf_pk uid (lat : map_val_ty) n_vers : iProp Σ :=
+Definition msv_Some (m : adtr_map_ty) vrf_pk uid pk n_vers : iProp Σ :=
   "#Hhist" ∷
     (∀ ver, ⌜ uint.Z ver < uint.Z (word.sub n_vers (W64 1)) ⌝ -∗
     ∃ label val,
     "#Hlabel" ∷ is_map_label vrf_pk uid ver label ∗
     "%Hlook_map" ∷ ⌜ m !! label = Some val ⌝) ∗
   "#Hlatest" ∷
-    (∃ lat_commit label,
-    "%Heq_ep" ∷ ⌜ lat.1 = lat_commit.1 ⌝ ∗
-    "#Hcommit" ∷ is_commit lat.2 lat_commit.2 ∗
+    (∃ ep commit label,
+    "#Hcommit" ∷ is_commit pk commit ∗
     "#Hlabel" ∷ is_map_label vrf_pk uid (word.sub n_vers (W64 1)) label ∗
-    "%Hlook_map" ∷ ⌜ m !! label = Some lat_commit ⌝) ∗
+    "%Hlook_map" ∷ ⌜ m !! label = Some (ep, commit) ⌝) ∗
   "#Hbound" ∷
     (∃ label,
     "#Hlabel" ∷ is_map_label vrf_pk uid n_vers label ∗
     "%Hlook_map" ∷ ⌜ m !! label = None ⌝).
 
-Lemma msv_Some_vers_agree_aux m vrf_pk uid lat0 n_vers0 lat1 n_vers1 :
+Lemma msv_Some_vers_agree_aux m vrf_pk uid pk0 n_vers0 pk1 n_vers1 :
   uint.Z n_vers0 < uint.Z n_vers1 →
-  msv_Some m vrf_pk uid lat0 n_vers0 -∗
-  msv_Some m vrf_pk uid lat1 n_vers1 -∗
+  msv_Some m vrf_pk uid pk0 n_vers0 -∗
+  msv_Some m vrf_pk uid pk1 n_vers1 -∗
   False.
 Proof.
   iIntros (?).
@@ -53,9 +52,9 @@ Proof.
     naive_solver.
 Qed.
 
-Lemma msv_Some_vers_agree m vrf_pk uid lat0 n_vers0 lat1 n_vers1 :
-  msv_Some m vrf_pk uid lat0 n_vers0 -∗
-  msv_Some m vrf_pk uid lat1 n_vers1 -∗
+Lemma msv_Some_vers_agree m vrf_pk uid pk0 n_vers0 pk1 n_vers1 :
+  msv_Some m vrf_pk uid pk0 n_vers0 -∗
+  msv_Some m vrf_pk uid pk1 n_vers1 -∗
   ⌜ n_vers0 = n_vers1 ⌝.
 Proof.
   iIntros "Hmsv0 Hmsv1".
@@ -66,8 +65,8 @@ Proof.
   word.
 Qed.
 
-Lemma msv_Some_nonzero_ver m vrf_pk uid lat n_vers :
-  msv_Some m vrf_pk uid lat n_vers -∗
+Lemma msv_Some_nonzero_ver m vrf_pk uid pk n_vers :
+  msv_Some m vrf_pk uid pk n_vers -∗
   ⌜ 0 < uint.Z n_vers ⌝.
 Proof.
   iNamed 1.
@@ -84,8 +83,8 @@ Definition msv_None (m : adtr_map_ty) vrf_pk uid : iProp Σ :=
   "#Hlabel" ∷ is_map_label vrf_pk uid (W64 0) label ∗
   "%Hlook_map" ∷ ⌜ m !! label = None ⌝.
 
-Lemma msv_Some_None_excl m vrf_pk uid lat n_vers :
-  msv_Some m vrf_pk uid lat n_vers -∗
+Lemma msv_Some_None_excl m vrf_pk uid pk n_vers :
+  msv_Some m vrf_pk uid pk n_vers -∗
   msv_None m vrf_pk uid -∗
   False.
 Proof.
@@ -103,31 +102,30 @@ Proof.
     naive_solver.
 Qed.
 
-(* TODO: should only talk about latest pk and leave existentially hidden. *)
-Definition msv γaudit vrf_pk (ep : w64) uid lat : iProp Σ :=
+Definition msv γaudit vrf_pk (ep : w64) uid opt_pk : iProp Σ :=
   ∃ m dig,
   "#Hlook_gs" ∷ mono_list_idx_own γaudit (uint.nat ep) (m, dig) ∗
-  "#Hmsv" ∷ match lat with
+  "#Hmsv" ∷ match opt_pk with
     | None => "#Hmsv" ∷ msv_None m vrf_pk uid
-    | Some lat' => ∃ n_vers, "#Hmsv" ∷ msv_Some m vrf_pk uid lat' n_vers
+    | Some pk => ∃ n_vers, "#Hmsv" ∷ msv_Some m vrf_pk uid pk n_vers
     end.
 
-Lemma msv_agree γ vrf_pk ep uid lat0 lat1 :
-  msv γ vrf_pk ep uid lat0 -∗
-  msv γ vrf_pk ep uid lat1 -∗
-  ⌜ lat0 = lat1 ⌝.
+Lemma msv_agree γ vrf_pk ep uid opt_pk0 opt_pk1 :
+  msv γ vrf_pk ep uid opt_pk0 -∗
+  msv γ vrf_pk ep uid opt_pk1 -∗
+  ⌜ opt_pk0 = opt_pk1 ⌝.
 Proof.
   iNamedSuffix 1 "0". iNamedSuffix 1 "1".
   iDestruct (mono_list_idx_agree with "Hlook_gs0 Hlook_gs1") as %?.
   simplify_eq/=.
-  destruct lat0 as [[??]|], lat1 as [[??]|]; [..|done];
+  destruct opt_pk0, opt_pk1; [..|done];
     iNamedSuffix "Hmsv0" "0"; iNamedSuffix "Hmsv1" "1".
   - iDestruct (msv_Some_vers_agree with "Hmsv0 Hmsv1") as %->.
     iNamedSuffix "Hmsv0" "0". iNamedSuffix "Hmsv1" "1".
     iClear "Hhist0 Hbound0 Hhist1 Hbound1".
     iNamedSuffix "Hlatest0" "0". iNamedSuffix "Hlatest1" "1".
     iDestruct (is_vrf_out_det with "Hlabel0 Hlabel1") as %->.
-    destruct lat_commit as [??]. simplify_eq/=.
+    simplify_eq/=.
     iDestruct (is_commit_inj with "Hcommit0 Hcommit1") as %?.
     by simplify_eq/=.
   - iDestruct (msv_Some_None_excl with "Hmsv0 Hmsv1") as "[]".
